src/pigeon.v
@@ -1,0 +1,10 @@
+Require Import ch2o.prelude.base.
+Require Import Coq.Lists.List.
+
+Theorem pigeonhole {X Ys: Type} `{Size (list X)} `{Size Ys} `{ElemOf X Ys} : forall (xs: list X) (ys: Ys),
+  base.NoDup xs ->
+  Forall (λ x, x ∈ ys) xs ->
+  size xs ≤ size ys.
+Proof.
+
+Admitted.
