src/subtyping.v
@@ -1,0 +1,226 @@
+Require Import Ast.
+Require Import ch2o.prelude.stringmap.
+Require Import ch2o.prelude.base.
+Require Import ch2o.prelude.list.
+Require Import Coq.Strings.String.
+Require Import Coq.Lists.List.
+Require Import Coq.Bool.Sumbool.
+Require Import pigeon.
+Require Import common.
+
+Class Subtype (A: Type) := subtype: program -> A -> A -> option unit.
+Instance subtype_cap : Subtype ecap := {
+  subtype P sub super :=
+    match sub, super with
+    | cap_iso_eph, _ => Some ()
+    | cap_iso, cap_iso => Some ()
+    | cap_ref, cap_ref => Some ()
+    | _, cap_tag => Some ()
+    | _, _ => None
+    end
+}.
+
+Definition assumes_wf (P: program) (assumes: list (string * string)) : Prop :=
+  ch2o.prelude.base.NoDup assumes ∧ Forall (λ a, a ∈ (P, P)) assumes.
+
+Program Fixpoint subtype_ty' (P: program) (assumes: list (string * string) | assumes_wf P assumes) (sub: ty) (super: ty)
+    {measure (size (P,P) - size (assumes: list (string * string)))} : option unit :=
+
+  let fix subclass (maxdepth: nat) (sub_name: string) (super_name: string) : option unit :=
+    match decide (elem_of (sub_name, super_name) (assumes: list (string * string))) with
+    | left _ => Some ()
+    | right HnotElem =>
+        if string_beq sub_name super_name
+        then Some () else
+
+        let fix nominal_subtype (is: list string) :=
+          match maxdepth, is with
+          | S maxdepth', i::is' =>
+              match subclass maxdepth' i super_name with
+              | Some () => Some ()
+              | None => nominal_subtype is'
+              end
+          | O, _ => None
+          | _, nil => None
+          end
+        in
+
+        is <- lookup_Is P sub_name;
+
+        if decide (is_Some (nominal_subtype is))
+        then Some () else
+
+        if decide (is_Some (lookup_P P sub_name) ∧ is_Some (lookup_P P super_name))
+        then
+          let assumes' := ((sub_name, super_name)::assumes) in
+
+          let fix args_subtype (sub_args: list (string * ty)) (super_args: list (string * ty)) :=
+            match sub_args, super_args with
+            | nil, nil => Some ()
+            | (_, sub_arg_ty)::sub_args', (_, super_arg_ty)::super_args' =>
+                _ <- subtype_ty' P assumes' sub_arg_ty super_arg_ty;
+
+                args_subtype sub_args' super_args'
+            | _, _ => None
+            end
+          in
+
+          let method_subtype (sub_method: func_stub) (super_method: func_stub) : option unit :=
+            let '(_, (sub_recv, sub_args, sub_retty)) := sub_method in
+            let '(_, (super_recv, super_args, super_retty)) := super_method in
+
+            _ <- subtype P (ecap_cap sub_recv) (ecap_cap super_recv); (* Covariant receiver capability *)
+            _ <- args_subtype super_args sub_args;                    (* Contravariant arguments *)
+            _ <- subtype_ty' P assumes' sub_retty super_retty;        (* Covariant return type *)
+            Some ()
+          in
+
+          let structural_subtype : option unit :=
+            super_ms <- lookup_Ms P 100 super_name;
+            sub_ms <- lookup_Ms P 100 sub_name;
+
+            _ <- mapM (λ m, m' <- sub_ms !! (fst m); method_subtype (fst m, m') m) super_ms;
+
+            Some ()
+          in
+
+          if decide (is_Some structural_subtype)
+          then Some () else
+          None
+        else None
+    end
+  in
+
+  match sub, super with
+  | ty_name name_sub cap_sub, ty_name name_super cap_super =>
+      _ <- subclass 100 name_sub name_super;
+      subtype P cap_sub cap_super
+
+  | ty_null, _ => Some ()
+  | _, ty_null => None
+  end.
+
+Next Obligation.
+unfold assumes_wf.
+destruct H2.
+split.
++ apply NoDup_cons_2.
+  exact HnotElem.
+  exact H2.
++ apply Forall_cons.
+  unfold elem_of, collection_cross_elem.
+  - split.
+    * apply lookup_P_is_some_elem_of2.
+      auto.
+    * apply lookup_P_is_some_elem_of2.
+      auto.
+  - exact H3.
+Defined.
+
+Next Obligation.
+destruct H2.
+assert ((size ((sub_name, super_name)::assumes)) <= size (P, P)).
+
+apply pigeonhole.
++ apply NoDup_cons_2.
+  exact HnotElem.
+  exact H2.
++ apply Forall_cons.
+  unfold elem_of, collection_cross_elem.
+  - split.
+    * apply lookup_P_is_some_elem_of2.
+      auto.
+    * apply lookup_P_is_some_elem_of2.
+      auto.
+  - exact H3.
++
+unfold size, list_size, Datatypes.length, collection_cross_size in H4.
+fold (Datatypes.length assumes) in H4.
+
+unfold size, list_size, Datatypes.length, collection_cross_size.
+fold (Datatypes.length assumes).
+fold (size P).
+
+omega.
+
+Defined.
+
+Next Obligation.
+split.
+intros.
+unfold not.
+intros.
+destruct H4.
+auto with *.
+unfold not.
+intros.
+destruct H4.
+auto with *.
+Defined.
+
+Next Obligation.
+split.
+intros.
+unfold not.
+intros.
+destruct H6.
+auto with *.
+unfold not.
+intros.
+destruct H6.
+auto with *.
+Defined.
+
+Next Obligation.
+unfold assumes_wf.
+destruct H4.
+split.
++ apply NoDup_cons_2.
+  exact HnotElem.
+  exact H4.
++ apply Forall_cons.
+  unfold elem_of, collection_cross_elem.
+  - split.
+    * apply lookup_P_is_some_elem_of2.
+      auto.
+    * apply lookup_P_is_some_elem_of2.
+      auto.
+  - exact H5.
+Defined.
+
+Next Obligation.
+destruct H4.
+assert ((size ((sub_name, super_name)::assumes)) <= size (P, P)).
+
+apply pigeonhole.
++ apply NoDup_cons_2.
+  exact HnotElem.
+  exact H4.
++ apply Forall_cons.
+  unfold elem_of, collection_cross_elem.
+  - split.
+    * apply lookup_P_is_some_elem_of2.
+      auto.
+    * apply lookup_P_is_some_elem_of2.
+      auto.
+  - exact H5.
++
+unfold size, list_size, Datatypes.length, collection_cross_size in H6.
+fold (Datatypes.length assumes) in H6.
+
+unfold size, list_size, Datatypes.length, collection_cross_size.
+fold (Datatypes.length assumes).
+fold (size P).
+
+omega.
+Defined.
+
+Program Instance subtype_ty : Subtype ty :=
+  fun P => subtype_ty' P nil.
+
+Next Obligation.
+unfold assumes_wf.
+split.
+apply NoDup_nil_2.
+apply Forall_nil.
+Qed.
